use corestepN in example, but without the juicy stuff

examples/step_if1_corestep.v
@@ -1,9 +1,3 @@
-(* This is an example showing how to use corestepN to step through a program.
-   corestepN is basically just N times cl_step plus juicy memory stuff.
-   If we use corestepN instead of our homemade star on top of cl_step, we have to deal
-   with juicy memory stuff, but we get lemmas from sepcomp.semantics_lemmas for free,
-   in particular those at the end of the file in sections corestepN and memstepN. *)
-
 Require Import veric.juicy_base.
 Require Import veric.juicy_mem veric.juicy_mem_lemmas veric.juicy_mem_ops.
 Require Import veric.res_predicates.
@@ -25,9 +19,8 @@ Require Import List. Import ListNotations.
 
 Require Import examples.if1.
 
-(* Inspired by veric.semax.jsafeN *)
-Definition stepN: genv -> nat -> corestate -> juicy_mem -> corestate -> juicy_mem -> Prop :=
-  corestepN (juicy_core_sem cl_core_sem).
+Definition stepN: genv -> nat -> corestate -> mem -> corestate -> mem -> Prop :=
+  corestepN cl_core_sem.
 
 Definition ge: genv := globalenv prog. (* prog is the concrete program in examples.if1 *)
 
@@ -36,9 +29,7 @@ Definition env0 : env := PTree.empty _.
 Definition temp_env0 : temp_env := 
   (PTree.Node PTree.Leaf (Some (Vptr (BinNums.xI 24) (Int.repr 0))) PTree.Leaf).
 
-(* Definition m0 := Memory.Mem.empty. *)
-
-Parameter m0: juicy_mem.
+Definition m0 := Memory.Mem.empty.
 
 Definition main_block: Values.block := ltac:(
   let o := eval hnf in (Globalenvs.Genv.find_symbol ge (Ctypes.prog_main prog)) in
@@ -62,38 +53,16 @@ Proof.
   intros. destruct (Int.eq_dec i i). reflexivity. exfalso. auto.
 Qed.
 
-Axiom admit_resource_decay_and_level: forall (m0: juicy_mem),
-  exists m1,
-  m_dry m0 = m_dry m1 /\
-  resource_decay (nextblock (m_dry m0)) (m_phi m0) (m_phi m1) /\
-  level m0 = S (level m1).
-
-(*
-Definition lvl_j := (@level juicy_mem juicy_mem_ageable).
-
-Definition lvl_phi := (@level rmap ag_rmap).
-*)
-
-(* Overview:
-   stepN is defined in this file to instantiate some parameters of
-   corestepN, which is, if instantiated with (juicy_core_sem cl_core_sem), defined in terms of
-   jstep, which is defined in terms of
-   corestep, which is defined in terms of
-   cl_step, which is the step relation we were using before in simple_ifc and in step_if1 *)
-
 Goal exists n eFinal teFinal mFinal, forall k,
   stepN ge n
         (State env0 temp_env0 ((Kseq (Scall None main_expr [])) :: k)) m0
         (State eFinal teFinal k) mFinal.
 Proof.
   exists 7%nat. do 3 eexists. intro k.
-  unfold stepN. unfold corestepN. unfold corestep. unfold juicy_core_sem.
+  unfold stepN. unfold corestepN. unfold corestep. simpl.
 
   (* call of main function *)
-  destruct (admit_resource_decay_and_level m0) as [m1 [E P]].
-  do 2 eexists. split.
-  { unfold jstep. refine (conj _ P).
-  { unfold corestep, cl_core_sem.
+  do 2 eexists. split. {
   eapply step_call_internal.
   - simpl. reflexivity.
   - constructor. simpl. reflexivity.
@@ -106,88 +75,57 @@ Proof.
   - repeat constructor; cbv; intros; repeat match goal with
     | H: _ \/ _ |- _ => destruct H
     end; auto; discriminate.
-  - rewrite E. constructor.
+  - constructor.
   - reflexivity.
-  } } {
+  } {
 
   (* bool b = true; *)
-  clear E P.
-  destruct (admit_resource_decay_and_level m1) as [m2 [E P]].
-  do 2 eexists. split.
-  { unfold jstep. refine (conj _ P).
-  { unfold corestep, cl_core_sem.
+  do 2 eexists. split. {
   simpl (fn_body f_main).
   repeat eapply step_seq.
-  rewrite E.
   eapply step_set.
   repeat econstructor.
-  } }
+  } {
 
   (* int n = 2; *)
-  clear E P.
-  destruct (admit_resource_decay_and_level m2) as [m3 [E P]].
-  do 2 eexists. split.
-  { unfold jstep. refine (conj _ P).
-  { unfold corestep, cl_core_sem.
+  do 2 eexists. split. {
   repeat eapply step_seq.
-  rewrite E.
   eapply step_set.
   repeat econstructor.
-  } }
+  } {
 
   (* int m = 3; *)
-  clear E P.
-  destruct (admit_resource_decay_and_level m3) as [m4 [E P]].
-  do 2 eexists. split.
-  { unfold jstep. refine (conj _ P).
-  { unfold corestep, cl_core_sem.
+  do 2 eexists. split. {
   repeat eapply step_seq.
-  rewrite E.
   eapply step_set.
   repeat econstructor.
-  } }
+  } {
 
   (* if-then-else *)
-  clear E P.
-  destruct (admit_resource_decay_and_level m4) as [m5 [E P]].
-  do 2 eexists. split.
-  { unfold jstep. refine (conj _ P).
-  { unfold corestep, cl_core_sem.
+  do 2 eexists. split. {
   repeat eapply step_seq.
-  rewrite E.
   eapply step_ifthenelse.
   - econstructor. reflexivity.
   - reflexivity.
-  } } {
+  } {
   simpl (if negb _ then Sset _ _ else _).
   rewrite Int.eq_false by (  rewrite Int.eq_false; intro; discriminate).
   simpl (if negb _ then Sset _ _ else _). 
 
   (* we're always in the then-branch *)
-  clear E P.
-  destruct (admit_resource_decay_and_level m5) as [m6 [E P]].
-  do 2 eexists. split.
-  { unfold jstep. refine (conj _ P).
-  { unfold corestep, cl_core_sem.
-  rewrite E.
+  do 2 eexists. split. {
   eapply step_set.
   repeat econstructor.
-  } } {
+  } {
 
   (* return res; *)
-  clear E P.
-  destruct (admit_resource_decay_and_level m6) as [m7 [E P]].
-  do 2 eexists. split.
-  { unfold jstep. refine (conj _ P).
-  { unfold corestep, cl_core_sem.
+  do 2 eexists. split. {
   eapply step_return.
   - simpl. reflexivity.
-  - simpl. rewrite E. reflexivity.
+  - simpl. reflexivity.
   - eexists. repeat constructor.
   - simpl. auto.
-  } } {
-    (* almost there: "reflexivity" complains:
-       cannot instantiate "?mFinal" because "m7" is not in its scope *)
-    admit.
-  } } } }
-Admitted.
+  } {
+    reflexivity.
+  } } } } } } }
+Qed.
